\documentclass[a3paper,12pt]{report}
\usepackage[margin=1in]{geometry}
\usepackage{amsmath}
\begin{document}
	\begin{center}
		\Large
		\textsc{Equations Used}\\\normalsize
	\end{center}
	\vspace{-3ex}
	\underline{\hspace{9.77in}}
	\begin{eqnarray}
		EI\frac{d^2\theta^*}{ds^{*2}} &=& \frac{1}{2}\rho u^2C_D\int_{s^*}^{l} \cos^2\theta\cos(\theta - \theta^*) ds + \frac{1}	{2}\rho u^2C_L\int_{s^*}^{l} \cos^2\theta\sin(\theta - \theta^*) ds\\
		\frac{d^2\theta^*}{ds^{*2}} &=& \frac{\rho u^2l}{2EI}\left[C_D\int_{s^*}^{1} \cos^2\theta\cos(\theta - \theta^*) ds + C_L\int_{s^*}^{1} \cos^2\theta\sin(\theta - \theta^*) ds	\right]\\
		\frac{d^2\theta^*}{ds^{*2}} &=& \frac{\rho u^2l}{2EI}\left[\int_{s^*}^{1} \cos^2\theta\left(C_D\cos(\theta - \theta^*) + C_L\sin(\theta - \theta^*)\right) ds	\right]\\
		\frac{d^2\theta^*}{ds^{*2}} &=& \frac{\rho u^2l}{2EI}\sqrt{C_D^2+C_L^2}\left[\int_{s^*}^{1} \cos^2\theta\left(\frac{C_D}{\sqrt{C_D^2+C_L^2}}\cos(\theta - \theta^*) + \frac{C_L}{\sqrt{C_D^2+C_L^2}}\sin(\theta - \theta^*)\right) ds	\right]\\
		\frac{d^2\theta^*}{ds^{*2}} &=& \frac{\rho u^2l}{2EI}\sqrt{C_D^2+C_L^2}\left[\int_{s^*}^{1} \cos^2\theta\sin\left(\theta - \theta^*+\sin^{-1}\left(\frac{C_D}{\sqrt{C_D^2+C_L^2} }\right)\right) ds\right]\\
		\frac{d^2\theta^*}{ds^{*2}} &=& a\left[\int_{s^*}^{1} \cos^2\theta\sin\left(\theta - \theta^*+\sin^{-1}\left(\frac{C_D}{\sqrt{C_D^2+C_L^2} }\right)\right) ds\right]\\
		\frac{d^3\theta^*}{ds^{*3}} &=& a\left[-\cos^2\theta^*\frac{C_D}{\sqrt{C_D^2+C_L^2} }-\int_{s^*}^{1} \cos^2\theta\cos\left(\theta - \theta^*+\sin^{-1}\left(\frac{C_D}{\sqrt{C_D^2+C_L^2} }\right)\right) ds\right]\\
		\frac{d^4\theta^*}{ds^{*4}} &=& a\left[2\cos\theta^*\sin\theta^*\frac{C_D}{\sqrt{C_D^2+C_L^2}}+ \cos^2\theta^*\frac{C_L}{\sqrt{C_D^2+C_L^2}}-\int_{s^*}^{1} \cos^2\theta\sin\left(\theta - \theta^*+\sin^{-1}\left(\frac{C_D}{\sqrt{C_D^2+C_L^2} }\right)\right) ds\right]\\
		\frac{d^4\theta^*}{ds^{*4}} &=& a\left[\sin2\theta^*\frac{C_D}{\sqrt{C_D^2+C_L^2}}+ \cos^2\theta^*\frac{C_L}{\sqrt{C_D^2+C_L^2}}\right]-\frac{d^2\theta^*}{ds^{*2}}\\
		\frac{d^4\theta^*}{ds^{*4}}+\frac{d^2\theta^*}{ds^{*2}} &=& \frac{a}{\sqrt{C_D^2+C_L^2}}\left[C_D\sin2\theta^*+ C_L\cos^2\theta^*\right]\\
		\frac{d^4\theta^*}{ds^{*4}}+\frac{d^2\theta^*}{ds^{*2}} &=& \frac{a}{\sqrt{C_D^2+C_L^2}}\left[\frac{C_L}{2}+ C_D\sin2\theta^*+ \frac{C_L}{2}\cos2\theta^*\right]\\
		\frac{d^4\theta^*}{ds^{*4}}+\frac{d^2\theta^*}{ds^{*2}} &=& \frac{a}{\sqrt{C_D^2+C_L^2}}\left[\frac{C_L}{2}+ \sqrt{C_D^2 + \frac{C_L^2}{4}}\left(\frac{C_D}{\sqrt{C_D^2 + \frac{C_L^2}{4}}}\sin2\theta^*+ \frac{C_L}{2\sqrt{C_D^2 + \frac{C_L^2}{4}}}\cos2\theta^*\right)\right]\\
		\frac{d^4\theta^*}{ds^{*4}}+\frac{d^2\theta^*}{ds^{*2}} &=& a\left(\lambda+ b\sin(2\theta^* + \mu)\right)
	\end{eqnarray}
where,\\
\raggedright
\begin{eqnarray*}
C_D &=& 1.95\\
C_L &=& 0.178\\
\lambda &=& \frac{C_L}{2\sqrt{C_D^2+C_L^2}}\\
 &=& 0.00454521\\
b &=& \frac{\sqrt{C_D^2 + \frac{C_L^2}{4}}}{\sqrt{C_D^2+C_L^2}}\\
 &=& 0.99689635\\
\mu &=& \sin^{-1}\left(\frac{C_L}{2\sqrt{C_D^2 + \frac{C_L^2}{4}}}\right)\\
 &=& 0.04561\\
\end{eqnarray*}
And the boundary conditions being,
\begin{eqnarray}
\theta^*(0)&=&0\\ 
\frac{d\theta^*}{ds^*}(1) &=& 0\\
\frac{d^2\theta^*}{ds^{*2}}(1) &=& 0\\
\frac{d^3\theta^*}{ds^{*3}}(1) &=& -a \frac{C_D}{\sqrt{C_D^2+C_L^2}}\cos^2\theta^*(1) \\
&=& -0.99585965a\cos^2\theta^*(1)
\end{eqnarray}

\end{document}